Preliminary spec for AES-GCTR encryption and some proven properties of the spec

src/crypto/aes/GCTR_s.fst
@@ -6,13 +6,15 @@ open FStar.Mul
 open AES_s
 open FStar.List.Tot.Base
 
+type gctr_plain = p:list quad32 { 256 * length p < nat32_max }
+
 let inc32 (cb:quad32) (i:int) = 
   Quad32 ((cb.lo + i) % nat32_max) cb.mid_lo cb.mid_hi cb.hi
 
-let rec gctr_encrypt_recursive (icb:quad32) (plain:list quad32 { 256 * length plain < nat32_max }) 
+let rec gctr_encrypt_recursive (icb:quad32) (plain:gctr_plain) 
 			       (alg:algorithm) (key:aes_key alg) (i:int) =
   match plain with
-  | [] -> Nil
+  | [] -> []
   | hd :: tl -> (quad32_xor hd (aes_encrypt alg key (inc32 icb i))) :: (gctr_encrypt_recursive icb tl alg key (i + 1))
   
 (*
@@ -32,6 +34,6 @@ let rec gctr_encrypt_recursive (icb:quad32) (plain:seq quad32 { 256 * length pla
 *)
 
 // length plain < nat32_max / 256 <= spec max of 2**39 - 256;
-let gctr_encrypt (icb:quad32) (plain:list quad32 { 256 * length plain < nat32_max }) (alg:algorithm) (key:aes_key alg) =
+let gctr_encrypt (icb:quad32) (plain:gctr_plain) (alg:algorithm) (key:aes_key alg) =
   gctr_encrypt_recursive icb plain alg key 0
   
