src/crypto/aes/GCTR_i.fst
@@ -1,0 +1,58 @@
+module GCTR_i
+
+open Types_s
+open FStar.Mul
+open FStar.List.Tot.Base
+open AES_s
+open GCTR_s 
+
+let rec gctr_encrypt_recursive_length (icb:quad32) (plain:gctr_plain) 
+				      (alg:algorithm) (key:aes_key alg) (i:int) : 
+  Lemma(length (gctr_encrypt_recursive icb plain alg key i) == length plain) =
+  match plain with 
+  | [] -> ()
+  | hd :: tl -> gctr_encrypt_recursive_length icb tl alg key (i + 1); 
+  ()
+  			
+let rec gctr_encrypt_length (icb:quad32) (plain:list quad32 { 256 * length plain < nat32_max }) 
+			     (alg:algorithm) (key:aes_key alg) : 
+  Lemma(length (gctr_encrypt icb plain alg key) == length plain) 
+  [SMTPat (length (gctr_encrypt icb plain alg key))]
+  =
+  gctr_encrypt_recursive_length icb plain alg key 0
+
+let rec nth_in_bounds_is_some (l:list 'a) (i:int) : Lemma
+  (requires 0 <= i /\ i < length l)
+  (ensures Some? (nth l i))
+  [SMTPat (nth l i)]
+=
+  if i = 0 then ()
+  else nth_in_bounds_is_some (Cons?.tl l) (i - 1)
+
+let nth_in_bounds (l:list 'a) (i:int {0 <= i /\ i < length l}) =
+  nth_in_bounds_is_some l i;
+  Some?.v (nth l i)
+
+let rec gctr_indexed (icb:quad32) (plain:gctr_plain) 
+		     (alg:algorithm) (key:aes_key alg) (i:int { 0 <= i /\ i < length plain }) : Lemma
+  (requires True)
+  (ensures (let cipher = gctr_encrypt icb plain alg key in
+	    length cipher == length plain /\
+	   (nth_in_bounds cipher i == quad32_xor (nth_in_bounds plain i) (aes_encrypt alg key (inc32 icb i) ))))
+=
+  if i = 0 then ()
+  else (assume False)//; gctr_indexed icb (Cons?.tl plain) alg key (i - 1)
+ 
+  
+(*
+let rec gctr_equivalence (icb:quad32) (plain:gctr_plain) 
+		     (alg:algorithm) (key:aes_key alg) (cipher:list quad32) : Lemma
+  (requires length cipher == length plain /\
+             (forall i . {:pattern nth cipher i} 0 <= i /\ i < length cipher ==> 
+	     nth_in_bounds cipher i == quad32_xor (nth_in_bounds plain i) (aes_encrypt alg key (inc32 icb i) )))
+  (ensures  cipher == gctr_encrypt icb plain alg key)
+=
+  match plain with
+  | [] -> ()
+  | hd :: tl -> gctr_equivalence icb tl alg key (Cons?.tl cipher)
+*)
